Trying to update ulib to use DM4F STATE_h

src/typechecker/dmff.fs
@@ -506,6 +506,10 @@ let is_monadic_comp c =
   | M _ -> true
   | N _ -> false
 
+
+// Temporarily used in is_non_dependent_arrow
+exception Not_found
+
 // ... the _ and * transformations from the definition language to F* ---------
 
 let rec mk_star_to_type mk env a =
