ulib/FStar.MRef.fst
@@ -9,38 +9,44 @@ let monotonic (a:Type) (b:reln a) =
   /\ (forall x y z. b x y /\ b y z ==> b x z)   (* transitive *)
 
 abstract let mref (a:Type) (b:reln a) = ref a
-val as_ref: #a:Type -> #b:reln a -> mref a b -> GTot (ref a)
-let as_ref #a #b m = m
+unfold val as_ref: #a:Type -> #b:reln a -> mref a b -> GTot (ref a)
+unfold let as_ref #a #b m = m
 
-val contains: #a:Type -> #b:reln a -> h:heap -> mref a b -> GTot bool
-let contains #a #b h m = Heap.contains h (as_ref m)
+unfold val contains: #a:Type -> #b:reln a -> h:heap -> mref a b -> GTot bool
+unfold let contains #a #b h m = Heap.contains h (as_ref m)
 
-val sel: #a:Type -> #b:reln a -> h:heap -> mref a b -> GTot a
-let sel #a #b h m = Heap.sel h (as_ref m)
+unfold val sel: #a:Type -> #b:reln a -> h:heap -> mref a b -> GTot a
+unfold let sel #a #b h m = Heap.sel h (as_ref m)
 
-val upd: #a:Type -> #b:reln a -> h:heap -> mref a b -> a -> GTot heap
-let upd #a #b h m v = Heap.upd h (as_ref m) v
+unfold val upd: #a:Type -> #b:reln a -> h:heap -> mref a b -> a -> GTot heap
+unfold let upd #a #b h m v = Heap.upd h (as_ref m) v
 
 abstract type token (#a:Type) (#b:reln a) (r:mref a b) (p:a -> Type) = True
 abstract type witnessed (p:heap -> Type) = True
 
-type fresh(#a:Type) (#b:reln a) (x:a) h0 (r:mref a b) h1 = 
+type fresh(#a:Type) (#b:reln a) (x:a) h0 (r:mref a b) h1 =
   not(contains h0 r) /\ contains h1 r /\ h1==upd h0 r x
+
+let test (h:heap) (b:reln int) (r:ref int) : Lemma (Heap.contains h r <==> contains #_ #b h r) = ()
+
 
 val alloc: #a:Type
         -> #b:reln a
         -> x:a{monotonic a b}
         -> ST (mref a b)
               (requires (fun _ -> True))
-              (fun h0 r h1 -> fresh x h0 r h1)
-let alloc #a #b x = ST.alloc x
+              (fun h0 (r, h1) -> fresh x h0 r h1)
+let alloc #a #b x = let h0 = ST.get () in let r = ST.alloc x in let h1 = ST.get () in
+assert (  not(Heap.contains h0 r) /\ Heap.contains h1 r /\ h1==Heap.upd h0 r x ) ;
+assert (fresh #_ #b x h0 r h1)  ; admit () ; r
+
 
 val read: #a:Type
        -> #b:reln a
        -> x:mref a b
        -> ST a
             (requires (fun h -> True))
-            (ensures (fun h0 v h1 -> h0==h1 /\ v==sel h0 x))
+            (ensures (fun h0 (v, h1) -> h0==h1 /\ v==sel h0 x))
 let read #a #b x = !x
 
 val write: #a:Type
@@ -49,7 +55,7 @@ val write: #a:Type
         -> v:a
         -> ST unit
               (requires (fun h0 -> b (sel h0 x) v))
-              (ensures (fun h0 _ h1 -> h1==upd h0 x v))
+              (ensures (fun h0 (_, h1) -> h1==upd h0 x v))
 let write #a #b x v = x := v
 
 let stable (#a:Type) (p:(a -> Type)) (b:reln a) = forall x y. p x /\ b x y ==> p y
@@ -59,7 +65,7 @@ val take_token: #a:Type
           -> p:(a -> Type)
           -> ST unit
                 (requires (fun h0 -> p (sel h0 m) /\ stable p b))
-                (ensures (fun h0 _ h1 -> h0==h1 /\ token m p))
+                (ensures (fun h0 (_, h1) -> h0==h1 /\ token m p))
 let take_token #a #b m p = ()
 assume val recall_token: #a:Type
                      -> #b:reln a
@@ -67,7 +73,7 @@ assume val recall_token: #a:Type
                      -> p:(a -> Type)
                      -> ST unit
                        (requires (fun _ ->  token m p))
-                       (ensures (fun h0 _ h1 -> h0==h1 /\ p (sel h1 m)))
+                       (ensures (fun h0 (_, h1) -> h0==h1 /\ p (sel h1 m)))
 
 let stable_on_heap (#a:Type) (#b:reln a) (r:mref a b) (p:(heap -> Type)) = 
   forall h0 h1. p h0 /\ b (sel h0 r) (sel h1 r) ==> p h1
@@ -75,7 +81,7 @@ let stable_on_heap (#a:Type) (#b:reln a) (r:mref a b) (p:(heap -> Type)) =
 assume val recall: p:(heap -> Type)
                 -> ST unit
                       (requires (fun _ ->  witnessed p))
-                      (ensures (fun h0 _ h1 -> p h1))
+                      (ensures (fun h0 (_, h1) -> p h1))
 
 val witness: #a:Type
           -> #b:reln a
@@ -83,5 +89,5 @@ val witness: #a:Type
           -> p:(heap -> Type)
           -> ST unit
                 (requires (fun h0 -> p h0 /\ stable_on_heap m p))
-                (ensures (fun h0 _ h1 -> h0==h1 /\ witnessed p))
+                (ensures (fun h0 (_, h1) -> h0==h1 /\ witnessed p))
 let witness #a #b m p = ()
