ulib/FStar.ST.fst
@@ -26,31 +26,36 @@ type modifies_none (h0:heap) (h1:heap) = modifies TSet.empty h0 h1
 let st_pre = st_pre_h heap
 let st_post a = st_post_h heap a
 let st_wp a = st_wp_h heap a
+
+
 new_effect_for_free STATE = STATE_h heap
-unfold let lift_div_state (a:Type) (wp:pure_wp a) (p:st_post a) (h:heap) = wp (fun a -> p a h)
+
+
+unfold let lift_div_state (a:Type) (wp:pure_wp a) (h:heap) (p:st_post a) = wp (fun a -> p (a, h))
+
 sub_effect DIV ~> STATE = lift_div_state
 
 effect State (a:Type) (wp:st_wp a) =
        STATE a wp
 effect ST (a:Type) (pre:st_pre) (post: (heap -> Tot (st_post a))) =
        STATE a
-             (fun (p:st_post a) (h:heap) -> pre h /\ (forall a h1. pre h /\ post h a h1 ==> p a h1))
+             (fun (h:heap) (p:st_post a) -> pre h /\ (forall a h1. pre h /\ post h (a, h1) ==> p (a, h1)))
 effect St (a:Type) =
-       ST a (fun h -> True) (fun h0 r h1 -> True)
+       ST a (fun h -> True) (fun h0 (r, h1) -> True)
 
 (* signatures WITHOUT permissions *)
 assume val recall: #a:Type -> r:ref a -> STATE unit
-                                         (fun 'p h -> Heap.contains h r ==> 'p () h)
+                                         (fun h 'p -> Heap.contains h r ==> 'p ((), h))
 
 assume val alloc:  #a:Type -> init:a -> ST (ref a)
                                            (fun h -> True)
-                                           (fun h0 r h1 -> not(contains h0 r) /\ contains h1 r /\ h1==upd h0 r init)
+                                           (fun h0 (r, h1) -> not(contains h0 r) /\ contains h1 r /\ h1==upd h0 r init)
 
 assume val read:  #a:Type -> r:ref a -> STATE a
-                                         (fun 'p h -> 'p (sel h r) h)
+                                         (fun h 'p -> 'p ((sel h r), h))
 
 assume val write:  #a:Type -> r:ref a -> v:a -> ST unit
                                                  (fun h -> True)
-                                                 (fun h0 x h1 -> h1==upd h0 r v)
+                                                 (fun h0 (x, h1) -> h1==upd h0 r v)
 
-assume val get: unit -> ST heap (fun h -> True) (fun h0 h h1 -> h0==h1 /\ h==h1)
+assume val get: unit -> ST heap (fun h -> True) (fun h0 (h, h1) -> h0==h1 /\ h==h1)
