ulib/reclaimable/FStar.ST.fst
@@ -15,7 +15,7 @@
 *)
 module FStar.ST
 #set-options "--max_fuel 0 --initial_fuel 0 --initial_ifuel 0 --max_ifuel 0"
-open FStar.Set
+open FStar.TSet
 open FStar.Heap
 type ref (a:Type) = Heap.ref a
 
@@ -27,47 +27,48 @@ let st_pre = st_pre_h heap
 let st_post a = st_post_h heap a
 let st_wp a = st_wp_h heap a
 new_effect_for_free STATE = STATE_h heap
-unfold let lift_div_state (a:Type) (wp:pure_wp a) (p:st_post a) (h:heap) = wp (fun a -> p a h)
+unfold let lift_div_state (a:Type) (wp:pure_wp a) (h:heap) (p:st_post a) = wp (fun a -> p (a, h))
 sub_effect DIV ~> STATE = lift_div_state
 
 effect State (a:Type) (wp:st_wp a) =
        STATE a wp
 effect ST (a:Type) (pre:st_pre) (post: (heap -> Tot (st_post a))) =
        STATE a
-             (fun (p:st_post a) (h:heap) -> pre h /\ (forall a h1. (pre h /\ post h a h1) ==> p a h1)) (* WP *)
+             (fun (h:heap) (p:st_post a) -> pre h /\ (forall a h1. (pre h /\ post h (a, h1)) ==> p (a, h1))) (* WP *)
 effect St (a:Type) =
-       ST a (fun h -> True) (fun h0 r h1 -> True)
+       ST a (fun h -> True) (fun h0 (r, h1) -> True)
 
 (* signatures WITH permissions *)
 assume val alloc: #a:Type -> init:a -> ST (ref a)
                                          (fun h -> True)
-                                         (fun h0 r h1 -> not(contains h0 r) /\ contains h1 r /\ h1==upd h0 r init)
+                                         (fun h0 (r, h1) -> not(contains h0 r) /\ contains h1 r /\ h1==upd h0 r init)
 
 assume val read: #a:Type -> r:ref a -> ST a
                                          (requires (fun h -> contains h r))
-                                         (ensures (fun h0 x h1 -> h0==h1 /\ x==sel h0 r))
+                                         (ensures (fun h0 (x, h1) -> h0==h1 /\ x==sel h0 r))
 
 assume val write: #a:Type -> r:ref a -> v:a -> ST unit
                                                  (requires (fun h -> contains h r))
-                                                 (ensures (fun h0 x h1 -> h1==upd h0 r v))
+                                                 (ensures (fun h0 (x, h1) -> h1==upd h0 r v))
 
 assume val op_Colon_Equals: #a:Type -> r:ref a -> v:a -> ST unit
                                                  (requires (fun h -> contains h r))
-                                                 (ensures (fun h0 x h1 -> h1==upd h0 r v))
+                                                 (ensures (fun h0 (x, h1) -> h1==upd h0 r v))
 
 assume val free: #a:Type -> r:ref a -> ST unit
          (requires (fun h -> contains h r))
-         (ensures (fun h0 x h1 -> modifies !{r} h0 h1 /\ not(contains h1 r)))
+         (ensures (fun h0 (x, h1) -> modifies !{r} h0 h1 /\ not(contains h1 r)))
 
-assume val get: unit -> State heap (fun 'post h -> 'post h h)
+assume val get: unit -> State heap (fun h 'post -> 'post (h, h))
+
 
 assume val forget_ST: #a:Type -> #b:(a -> Type)
   -> #req:(a -> heap -> Type)
-  -> #ens:(x:a -> heap -> b x -> heap -> Type)
+  -> #ens:(x:a -> heap -> (b x) * heap -> Type)
   -> $f:(x:a -> ST (b x) (req x) (ens x))
   -> Pure (x:a -> Div (b x)
                  (requires (forall h. req x h))
-                 (ensures (fun (y:b x) -> exists h0 h1. ens x h0 y h1)))
+                 (ensures (fun (y:b x) -> exists h0 h1. ens x h0 (y, h1))))
           (requires (forall (x:a) (y:b x) h h'.
-                        (req x h /\ ens x h y h' ==> modifies !{} h h')))
+                        (req x h /\ ens x h (y, h') ==> modifies !{} h h')))
           (ensures (fun _ -> True))
